WIP: trying to define the 'ThreadLinking' operation

common/SmallstepMulti.v
@@ -8,32 +8,170 @@ Require Import LanguageInterface.
 Require Import Integers.
 Require Import Smallstep.
 Require Import SmallstepClosed.
-Import Values Maps Memory AST.
+Require Import Values Maps Memory AST.
 
+Module NatIndexed.
+    Definition t := nat.
+
+    Fixpoint index (n : nat) : positive :=
+      match n with
+      |O => 1%positive
+      |S n => 1 + index n
+      end.
+
+    (*wrong, fix it later*)
+    Definition index_rev (p:positive) : nat :=
+      Pos.to_nat p.
+
+    Lemma t_positive_t : forall (n:nat), index_rev (index n) = n.
+    Admitted.
+
+    Lemma positive_t_positive : forall (p:positive), index(index_rev p) = p.
+    Admitted.
+
+    Lemma index_inj : forall (x y : nat), index x = index y -> x = y.
+    Admitted.
+
+    Definition eq := Nat.eq_dec.
+End NatIndexed.
+
+Module NatMap := IRMap(NatIndexed).
+    
 Section MultiThread.
 
-  Context {liA liB : language_interface}.
+  Context {OpenS : semantics li_c li_c}.
 
-  Context {OS : semantics liA liB}.
+  Definition local_state := state OpenS.
 
-  Definition local_state := state OS.
+  (* Maybe should be somehow added into open semantics *)
+  Variable initial_query : query li_c.
+  Variable final_reply : int -> reply li_c -> Prop.
 
-  Variable initial_query : query liB.
+  (* should be derived from skel of OpenS
 
+     and allocate blocks for pthread primitives
+  *)
+  Variable initial_se : Genv.symtbl.
+  
+  Definition OpenLTS := activate OpenS initial_se.
+  Definition ClosedS := Closed.close_semantics initial_query final_reply OpenS initial_se.
   
   (* The global state of concurrent semantics *)
 
   (* problem : how to deal with "thread variable" *)
 
-  Definition state := list local_state.
+  (* Definition state := list local_state. *)
 
-  Closed.semantics
+
+  Variable get_gmem : local_state -> mem.
+  Variable set_gmem : mem -> local_state -> local_state.
+
+  Definition tid_mem (m:mem) : nat :=
+    Mem.tid (Mem.support m).
+
+  Definition stacks_mem (m:mem) :=
+    Mem.stacks (Mem.support m).
+
+  (* Definition and operations of global state *)
+
+    Record state : Type := mk_gstate
+    {
+      threads: NatMap.t (option local_state);
+      cur_tid : nat;
+      next_tid : nat;
+      (* atom_bit : bool; *)
+
+      (* tid_gmem : exists ls, NatMap.get cur_tid threads = Some ls /\
+                         tid_mem (get_gmem ls) = cur_tid /\
+                         length (stacks_mem (get_gmem ls)) = next_tid; *)
+    }.
+
+  Definition empty_threads : NatMap.t (option local_state) := NatMap.init None.
+  (* Definition initial_threads (ls :local_state) := NatMap.set 1%nat (Some ls) empty_threads.
+  Program Definition single_state (ls: local_state) := mk_gstate (initial_threads ls) 1%nat 2%nat false. *)
+
+  
+  Definition update_threads (s : state) (t: NatMap.t (option local_state)) :=
+    mk_gstate t (cur_tid s) (next_tid s) .
+
+  Variable yield_strategy : state -> nat.
+  Axiom yield_strategy_range : forall s, (1 < yield_strategy s < (next_tid s))%nat.
+  (*some other properties may be added here, such as only point to active threads *)
+
+  (* We transfer to thread tid' and update its local_state to ls (synchronize the global memory for it) *)
+  Definition yield_state (s : state) (ls : local_state): state :=
+    match s with
+      mk_gstate threads cid nid =>
+        let tid' := yield_strategy s in
+        let threads' := NatMap.set tid' (Some ls) threads in
+      mk_gstate threads' tid' nid
+    end.
+
+  
+  (* problem here, we need some proofs about initial local_state for this initial gstate
+   *)
+
+  Definition genvtype := Smallstep.genvtype OpenLTS.
+  
   (** Initial state of Concurrent semantics *)
 
   (* We need a "query" to the main function of the semantics *)
   (* Including the initial global memory*)
 
+  Inductive initial_state : state -> Prop :=
+  |initial_state_intro : forall ls s,
+      cur_tid s = 1%nat -> next_tid s = 2%nat ->
+      NatMap.get 1%nat (threads s) = Some ls ->
+      (Closed.initial_state ClosedS) ls ->
+      initial_state s.
 
+  (** Final state of Concurrent semantics *)
+  Inductive final_state : state -> int -> Prop :=  
+  |final_state_intro : forall ls i s,
+      cur_tid s = 1%nat ->
+      NatMap.get 1%nat (threads s) = Some ls ->
+      final_state s i.
+
+  Definition yield_id := 1001%positive.
+  Definition yield_sig := mksignature nil Tvoid cc_default.
   
-
+  Inductive query_is_yield : query li_c -> Prop :=
+  |yield_intro : forall b m,
+    Genv.find_symbol initial_se yield_id = Some b ->
+    query_is_yield (cq (Vptr b Ptrofs.zero) yield_sig nil m).
+  
+  Inductive step : genvtype -> state -> trace -> state -> Prop :=
+  |step_local : forall ge ls1 t ls2 tid s s' threads',
+      let threads := threads s in
+      NatMap.get tid threads = Some ls1 ->
+      Smallstep.step OpenLTS ge ls1 t ls2 ->
+      threads' = NatMap.set tid (Some ls2) threads ->
+      s' = update_threads s threads ->
+      step ge s t s'
+  |step_thread_yield : forall ge s tid s' tid' gmem ls ls1 ls1' q,
+      NatMap.get tid (threads s) = Some ls ->
+      at_external OpenLTS ls q ->
+      query_is_yield q ->
+      cq_mem q = gmem ->
+      NatMap.get tid' (threads s) = Some ls1 ->
+      set_gmem gmem ls1 = ls1' ->
+      yield_strategy s = tid' ->      
+      yield_state s ls1' = s' ->
+      step ge s E0 s'.
+  |step_thread_create : ge s tid s' q,
+      NatMap.get tid (threads s) = Some ls ->
+      at_external OpenLTS ls q ->
+      query_is_create q ->
+      
+      
+      step ge s E0 s'.
+           
+      
+  (* problem : how to simultaneously update the memory for all threads *)
+  |Step_lock
+  |Step_unlock
+  |Step_thread_create
+     
+  |Step_thread_join
+   
   
